Lemmas/Instances.lean
@@ -1,0 +1,124 @@
+module
+
+public import Init.Meta
+
+import all Parser.Basic
+import all Parser.Error
+import all Parser.Parser
+import all Parser.Prelude
+import all Parser.Stream
+
+public import Std.Tactic.Do
+public import Std.Tactic.Do.Syntax
+
+public import Lemmas.Basic
+
+open Lean Lean.Syntax Parser Parser.Char
+
+open Std.Do
+
+@[expose] public section
+
+namespace Parser
+
+/-! WP instance of SimpleParser σ τ -/
+
+instance [Parser.Stream σ τ] : LawfulMonad (SimpleParser σ τ) where
+  id_map := by
+    intros
+    simp [Functor.map, bind, pure]
+    apply funext
+    intros
+    split <;> grind
+  map_const := by intros; rfl
+  seqLeft_eq := by
+    intros
+    simp [Functor.map, SeqLeft.seqLeft]
+    apply funext
+    intros
+    simp [bind, pure, Seq.seq]
+    split
+    · split
+      · split
+        · split
+          · expose_names; simp_all; rw [← heq_2.right]; grind
+          · grind
+        · grind
+      · grind
+    · grind
+  seqRight_eq := by
+    intros
+    simp [Functor.map, SeqRight.seqRight]
+    apply funext
+    intros
+    simp [bind, pure, Seq.seq]
+    split
+    · split
+      · split
+        · split
+          · expose_names; simp_all; rw [← heq_2.right]; simp [id]; grind
+          · grind
+        · grind
+      · grind
+    · grind
+  pure_seq := by simp [Seq.seq, Functor.map, pure, bind]
+  bind_pure_comp := by simp [bind, Functor.map, pure]
+  bind_map := by
+    intros
+    simp [Seq.seq, bind, pure, Functor.map]
+    apply funext
+    intros
+    grind
+  pure_bind := by simp [bind, pure]
+  bind_assoc := by
+    simp [bind, pure]
+    intros
+    apply funext
+    intros
+    grind
+
+instance SimpleParser.instWP [Parser.Stream σ τ]
+    : WP (SimpleParser σ τ) (.except (Parser.Error.Simple σ τ) (.arg σ .pure)) where
+  wp x :=
+    { trans := fun Q s => match x.run s with
+        | .ok s' a => Q.1 a s'
+        | .error s' e => Q.2.1 e s'
+      conjunctiveRaw := by
+        intro _ _
+        apply SPred.bientails.of_eq
+        ext s
+        dsimp
+        cases (x.run s) <;> simp
+    }
+
+instance SimpleParser.instWPMonad [Parser.Stream σ τ]
+    : WPMonad (SimpleParser σ τ) (.except (Parser.Error.Simple σ τ) (.arg σ .pure)) where
+  wp_pure a := by
+    ext Q : 1; simp only [wp, PredTrans.apply, pure]; rfl
+  wp_bind x f := by
+    ext Q : 2
+    simp only [wp, PredTrans.apply_Bind_bind, Parser.run]
+    simp only [PredTrans.apply]
+    simp only [bind, pure]
+    grind
+
+theorem SimpleParser.of_wp_run_eq {α} [Parser.Stream σ τ]
+  {x : Parser.Result (Error.Simple σ τ) σ α} {prog : SimpleParser σ τ α} (h : Parser.run prog s = x)
+  (P : Parser.Result (Error.Simple σ τ) σ α → Prop) :
+    (⊢ₛ wp⟦prog⟧ post⟨fun a s' => ⌜P (Parser.Result.ok s' a)⌝,
+                     fun e s' => ⌜P (Parser.Result.error s' e)⌝⟩ s) → P x := by
+  intro hspec
+  simp only [wp, PredTrans.apply] at hspec
+  split at hspec
+  case h_1 a s' heq => rw[← heq] at hspec; exact h ▸ hspec True.intro
+  case h_2 e s' heq => rw[← heq] at hspec; exact h ▸ hspec True.intro
+
+theorem SimpleParser.of_wp_eq [Parser.Stream σ τ]  (x : SimpleParser σ τ α)
+  {P : σ → SPred PostShape.pure.args}
+  {Q : (α → Assertion (PostShape.except (Error.Simple σ τ) (PostShape.arg σ PostShape.pure)))
+      × ExceptConds (PostShape.except (Error.Simple σ τ) (PostShape.arg σ PostShape.pure))}
+    (h : P ⊢ₛ wp⟦x⟧ Q) (it : σ) (hp : (P it).down)
+    : (match x it with | .ok s a => Q.1 a s | .error s e => Q.2.1 e s).down := by
+  simp [wp, PredTrans.apply, Parser.run] at h
+  have := h it hp
+  grind
