Lemmas/String/Basic.lean
@@ -1,0 +1,19 @@
+module
+
+import Init.Meta
+
+import all Init.Data.String.Basic
+
+public section
+
+namespace Parser.String.Slice
+
+@[simp] theorem castSliceStartInclusive (s1 s2 : String.Slice) (h1 : s1.str = s2.str)
+  (h2 : s1.startInclusive.offset = s2.startInclusive.offset)
+    : s1.startInclusive.cast h1 = s2.startInclusive := by
+  exact (String.Pos.ext h2)
+
+@[simp] theorem castSliceEndExclusive (s1 s2 : String.Slice) (h1 : s1.str = s2.str)
+  (h2 : s1.endExclusive.offset = s2.endExclusive.offset)
+    : s1.endExclusive.cast h1 = s2.endExclusive := by
+  exact (String.Pos.ext h2)
